theories/Semantics.v
@@ -1,6 +1,10 @@
 Require Import sflib.
 Require Import Universe.
 
+Set Implicit Arguments.
+
+
+
 Inductive sort: Type :=
 | angelic
 | demonic
@@ -13,7 +17,62 @@ Record semantics : Type := Semantics_gen {
   step : state -> option event -> state -> Prop;
   initial_state: state;
   state_sort: state -> sort;
-  wf_vis: forall st0 (VIS: state_sort st0 = vis), exists ! ev st1, step st0 (Some ev) st1;
+  (* wf_vis: forall st0 (VIS: state_sort st0 = vis), exists ! ev st1, step st0 (Some ev) st1; *)
+  (* wf_vis: forall st0 (VIS: state_sort st0 = vis), exists ev st1, step st0 (Some ev) st1; *)
+  wf_vis: forall
+      st0 ev0 ev1 st1 st2
+      (VIS: state_sort st0 = vis)
+      (STEP: step st0 ev0 st1)
+      (STEP: step st0 ev1 st2)
+    ,
+      ev0 = ev1 /\ st1 = st2;
   wf_angelic: forall st0 ev st1 (VIS: state_sort st0 = angelic) (STEP: step st0 ev st1), ev = None;
   wf_demonic: forall st0 ev st1 (VIS: state_sort st0 = demonic) (STEP: step st0 ev st1), ev = None;
 }.
+
+Section SEM.
+Variable L: semantics.
+
+Inductive tstar (st0: L.(state)) (P: L.(state) -> Prop): Prop :=
+| tstar_refl
+    (PROP: P st0)
+  :
+    tstar st0 P
+| tstar_demonic
+    (SRT: L.(state_sort) st0 = demonic)
+    (STEP: exists st1 (STEP: L.(step) st0 None st1), <<TL: tstar st1 P>>)
+  :
+    tstar st0 P
+| tstar_angelic
+    (SRT: L.(state_sort) st0 = angelic)
+    (STEP: forall st1 (STEP: L.(step) st0 None st1), <<TL: tstar st1 P>>)
+  :
+    tstar st0 P
+.
+
+Theorem tstar_ind2 :
+forall P : state L -> (state L -> Prop) -> Prop,
+(forall (st0 : state L) (P0 : state L -> Prop), P0 st0 -> P st0 P0) ->
+(forall (st0 : state L) (P0 : state L -> Prop),
+ state_sort L st0 = demonic ->
+ (exists (st1 : state L) (_ : step L st0 None st1), <<TL: tstar st1 P0 >> /\ <<IH: P st1 P0>>) -> P st0 P0) ->
+(forall (st0 : state L) (P0 : state L -> Prop),
+ state_sort L st0 = angelic ->
+ (forall st1 : state L, step L st0 None st1 -> <<TL: tstar st1 P0 >>) ->
+ (forall st1 : state L, step L st0 None st1 -> P st1 P0) -> P st0 P0) ->
+forall (st0 : state L) (P0 : state L -> Prop), tstar st0 P0 -> P st0 P0.
+Proof.
+  fix IH 7. i.
+  inv H2.
+  - eapply H; eauto.
+  - eapply H0; eauto. des. esplits; eauto. eapply IH; eauto.
+  - eapply H1; eauto. ii. exploit STEP; eauto. i. esplits; eauto. eapply IH; eauto.
+Qed.
+
+Definition is_leaf (st0: L.(state)): bool :=
+  match L.(state_sort) st0 with
+  | final | vis => true
+  | _ => false
+  end
+.
+End SEM.
