lib/sflib.v
@@ -6,7 +6,7 @@
 (* *********************************************************************)
 
 (** This file collects a number of basic lemmas and tactics for better
-    proof automation, structuring large proofs, or rewriting.  Most of
+    proof automation, structuring large proofs, or rewriting.  Most of 
     the rewriting support is ported from ssreflect. *)
 
 (** Symbols starting with [sflib__] are internal. *)
@@ -53,28 +53,28 @@ Hint Resolve sflib__true_is_true sflib__not_false_is_true.
 
 (** Set up for basic simplification *)
 
-Create HintDb sflib discriminated.
+Create HintDb sflib discriminated. 
 
 (** Adaptation of the ss-reflect "[done]" tactic. *)
 
-Ltac sflib__basic_done :=
+Ltac sflib__basic_done := 
   solve [trivial with sflib | apply sym_equal; trivial | discriminate | contradiction].
 
 Ltac done := unfold not in *; trivial with sflib; hnf; intros;
-  solve [try sflib__basic_done; split;
-         try sflib__basic_done; split;
-         try sflib__basic_done; split;
-         try sflib__basic_done; split;
+  solve [try sflib__basic_done; split; 
+         try sflib__basic_done; split; 
+         try sflib__basic_done; split; 
+         try sflib__basic_done; split; 
          try sflib__basic_done; split; sflib__basic_done
     | match goal with H : _ -> False |- _ => solve [case H; trivial] end].
 
 (** A variant of the ssr "done" tactic that performs "eassumption". *)
 
 Ltac edone := try eassumption; trivial; hnf; intros;
-  solve [try eassumption; try sflib__basic_done; split;
-         try eassumption; try sflib__basic_done; split;
-         try eassumption; try sflib__basic_done; split;
-         try eassumption; try sflib__basic_done; split;
+  solve [try eassumption; try sflib__basic_done; split; 
+         try eassumption; try sflib__basic_done; split; 
+         try eassumption; try sflib__basic_done; split; 
+         try eassumption; try sflib__basic_done; split; 
          try eassumption; try sflib__basic_done; split;
          try eassumption; sflib__basic_done
     | match goal with H : ~ _ |- _ => solve [case H; trivial] end].
@@ -130,7 +130,7 @@ Tactic Notation "hinv" ident(a) ident(b) :=
   (hinv a; hinv b).
 Tactic Notation "hinv" ident(a) ident(b) ident(c) :=
   (hinv a; hinv b c).
-Tactic Notation "hinv" ident(a) ident(b) ident(c) ident(d) :=
+Tactic Notation "hinv" ident(a) ident(b) ident(c) ident(d) := 
   (hinv a b; hinv c d).
 
 Ltac hinvc x := hinv x; clear x.
@@ -141,9 +141,9 @@ Tactic Notation "hinvc" ident(a) ident(b) :=
   (hinvc a; hinvc b).
 Tactic Notation "hinvc" ident(a) ident(b) ident(c) :=
   (hinvc a; hinvc b c).
-Tactic Notation "hinvc" ident(a) ident(b) ident(c) ident(d) :=
+Tactic Notation "hinvc" ident(a) ident(b) ident(c) ident(d) := 
   (hinvc a b; hinvc c d).
-Tactic Notation "hinvc" ident(a) ident(b) ident(c) ident(d) ident(e) :=
+Tactic Notation "hinvc" ident(a) ident(b) ident(c) ident(d) ident(e) := 
   (hinvc a b c; hinvc d e).
 
 Ltac simpls  := simpl in *; try done.
@@ -176,7 +176,8 @@ Ltac autos   := clarsimp; auto with sflib.
 
 Definition  NW A (P: () -> A) : A := P ().
 
-Notation "<< x : t >>" := (NW (fun x => (t):Prop)) (at level 80, x ident, no associativity).
+(* Notation "<< x : t >>" := (NW (fun x => (t):Prop)) (at level 80, x ident, no associativity). *)
+Notation "<< x : t >>" := (NW (fun x => (t))) (at level 80, x ident, no associativity).
 Notation "<< t >>" := (NW (fun _ => t)) (at level 79, no associativity).
 Notation "<< t >>" := (NW (fun _ => (t):Prop)) (at level 79, no associativity).
 
@@ -190,17 +191,17 @@ Ltac get_concl := lazymatch goal with [ |- ?G ] => G end.
 Ltac des1 :=
   match goal with
     | H : NW _ |- _ => red in H
-    | H : exists x, NW (fun y => _) |- _ =>
+    | H : exists x, NW (fun y => _) |- _ => 
       let x' := fresh x in let y' := fresh y in destruct H as [x' y']; red in y'
-    | H : exists x, ?p |- _ =>
+    | H : exists x, ?p |- _ => 
       let x' := fresh x in destruct H as [x' H]
-    | H : ?p /\ ?q |- _ =>
+    | H : ?p /\ ?q |- _ => 
       let x' := match p with | NW (fun z => _) => fresh z | _ => H end in
       let y' := match q with | NW (fun z => _) => fresh z | _ => fresh H end in
       destruct H as [x' y'];
       match p with | NW _ => red in x' | _ => idtac end;
       match q with | NW _ => red in y' | _ => idtac end
-    | H : ?p <-> ?q |- _ =>
+    | H : ?p <-> ?q |- _ => 
       let x' := match p with | NW (fun z => _) => fresh z | _ => H end in
       let y' := match q with | NW (fun z => _) => fresh z | _ => fresh H end in
       destruct H as [x' y'];
@@ -236,17 +237,17 @@ Ltac desc :=
 Ltac nbdes1 :=
   match goal with
     | H : NW _ |- _ => red in H
-    | H : exists x, NW (fun y => _) |- _ =>
+    | H : exists x, NW (fun y => _) |- _ => 
       let x' := fresh x in let y' := fresh y in destruct H as [x' y']; red in y'
-    | H : exists x, ?p |- _ =>
+    | H : exists x, ?p |- _ => 
       let x' := fresh x in destruct H as [x' H]
-    | H : ?p /\ ?q |- _ =>
+    | H : ?p /\ ?q |- _ => 
       let x' := match p with | NW (fun z => _) => fresh z | _ => H end in
       let y' := match q with | NW (fun z => _) => fresh z | _ => fresh H end in
       destruct H as [x' y'];
       match p with | NW _ => red in x' | _ => idtac end;
       match q with | NW _ => red in y' | _ => idtac end
-    | H : ?p <-> ?q |- _ =>
+    | H : ?p <-> ?q |- _ => 
       let x' := match p with | NW (fun z => _) => fresh z | _ => H end in
       let y' := match q with | NW (fun z => _) => fresh z | _ => fresh H end in
       destruct H as [x' y'];
@@ -269,17 +270,17 @@ Ltac forall_split :=
 Definition _HID_ (A : Type) (a : A) := a.
 
 Ltac hdesHi H P x y :=
-  let FF := fresh "__hdesfalse__" in
-  let TMP := fresh "__hdesHi__" in
-  let P1 := fresh "__hdesHi__" in
-  let P2 := fresh "__hdesHi__" in
+  let FF := fresh "__hdesfalse__" in 
+  let TMP := fresh "__hdesHi__" in 
+  let P1 := fresh "__hdesHi__" in 
+  let P2 := fresh "__hdesHi__" in 
     evar (P1 : Prop); evar (P2 : Prop);
     assert (TMP: False -> P) by
       (intro FF; forall_split;
          [ let G := get_concl in set (TMP := G); revert P1; instantiate (1:=G)
          | let G := get_concl in set (TMP := G); revert P2; instantiate (1:=G) ];
        destruct FF);
-    try clear TMP;
+    try clear TMP; 
     try (try (match goal with [Def := ?G : _ |- _] =>
               match Def with P1 =>
               match goal with [_ : G |- _] => fail 4 end end end);
@@ -288,35 +289,35 @@ Ltac hdesHi H P x y :=
     try (try (match goal with [Def := ?G : _ |- _] =>
               match Def with P2 =>
               match goal with [_ : G |- _] => fail 4 end end end);
-         assert (y: P2) by (unfold P2; repeat (let x := fresh "__xhj__" in intro x; specialize (H x)); apply H));
+         assert (y: P2) by (unfold P2; repeat (let x := fresh "__xhj__" in intro x; specialize (H x)); apply H)); 
     try unfold P2 in y; try clear P2;
     fold (_HID_ P) in H;
     try clear H.
 
 Ltac hdesHP H P :=
   let H' := fresh H in let H'' := fresh H in
-  match P with
-  | context[ NW (fun x => _) /\ NW (fun y => _) ] =>
+  match P with 
+  | context[ NW (fun x => _) /\ NW (fun y => _) ] => 
     let x' := fresh x in let y' := fresh y in
     hdesHi H P x' y'; red in x'; red in y'
-  | context[ NW (fun x => _) /\ _ ] =>
+  | context[ NW (fun x => _) /\ _ ] => 
     let x' := fresh x in
     hdesHi H P x' H'; red in x'
-  | context[ _ /\ NW (fun y => _) ] =>
+  | context[ _ /\ NW (fun y => _) ] => 
     let y' := fresh y in
     hdesHi H P H' y'; red in y'
-  | context[ _ /\ _ ] =>
+  | context[ _ /\ _ ] => 
     hdesHi H P H' H''
   | context[ NW (fun x => _) <-> NW (fun y => _) ] =>
     let x' := fresh x in let y' := fresh y in
     hdesHi H P x' y'; red in x'; red in y'
-  | context[ NW (fun x => _) <-> _ ] =>
+  | context[ NW (fun x => _) <-> _ ] => 
     let x' := fresh x in
     hdesHi H P x' H'; red in x'
-  | context[ _ <-> NW (fun y => _) ] =>
+  | context[ _ <-> NW (fun y => _) ] => 
     let y' := fresh y in
     hdesHi H P H' y'; red in y'
-  | context[ _ <-> _ ] =>
+  | context[ _ <-> _ ] => 
     hdesHi H P H' H''
   end.
 
@@ -332,32 +333,33 @@ Ltac hdesF P :=
     let P' := eval cbv beta in (fun p : sigT ty => f (projT1 p) (projT2 p)) in
       hdesF P'
   end.
-Ltac hdes :=
-  repeat match goal with | H : ?P |- _ => hdesF (fun _ : unit => P); hdesHP H P end;
+
+Ltac hdes := 
+  repeat match goal with | H : ?P |- _ => hdesF (fun _ : unit => P); hdesHP H P end; 
   unfold _HID_ in *.
 *)
 
 Ltac hdesF P :=
-  match P with | _ /\ _ => idtac | _ <-> _ => idtac | forall _, _ =>
-  match P with | forall _, _ /\ _ => idtac | forall _, _ <-> _ => idtac | forall _ _, _ =>
+  match P with | _ /\ _ => idtac | _ <-> _ => idtac | forall _, _ => 
+  match P with | forall _, _ /\ _ => idtac | forall _, _ <-> _ => idtac | forall _ _, _ => 
   match P with | forall _ _, _ /\ _ => idtac | forall _ _, _ <-> _ => idtac | forall _ _ _, _ =>
-  match P with | forall _ _ _, _ /\ _ => idtac | forall _ _ _, _ <-> _ => idtac | forall _ _ _ _, _ =>
+  match P with | forall _ _ _, _ /\ _ => idtac | forall _ _ _, _ <-> _ => idtac | forall _ _ _ _, _ => 
   match P with | forall _ _ _ _, _ /\ _ => idtac | forall _ _ _ _, _ <-> _ => idtac | forall _ _ _ _ _, _ =>
-  match P with | forall _ _ _ _ _, _ /\ _ => idtac | forall _ _ _ _ _, _ <-> _ => idtac | forall _ _ _ _ _ _, _ =>
-  match P with | forall _ _ _ _ _ _, _ /\ _ => idtac | forall _ _ _ _ _ _, _ <-> _ => idtac | forall _ _ _ _ _ _ _, _ =>
-  match P with | forall _ _ _ _ _ _ _, _ /\ _ => idtac | forall _ _ _ _ _ _ _, _ <-> _ => idtac | forall _ _ _ _ _ _ _ _, _ =>
+  match P with | forall _ _ _ _ _, _ /\ _ => idtac | forall _ _ _ _ _, _ <-> _ => idtac | forall _ _ _ _ _ _, _ => 
+  match P with | forall _ _ _ _ _ _, _ /\ _ => idtac | forall _ _ _ _ _ _, _ <-> _ => idtac | forall _ _ _ _ _ _ _, _ => 
+  match P with | forall _ _ _ _ _ _ _, _ /\ _ => idtac | forall _ _ _ _ _ _ _, _ <-> _ => idtac | forall _ _ _ _ _ _ _ _, _ => 
   match P with | forall _ _ _ _ _ _ _ _, _ /\ _ => idtac | forall _ _ _ _ _ _ _ _, _ <-> _ => idtac | forall _ _ _ _ _ _ _ _ _, _ =>
-  match P with | forall _ _ _ _ _ _ _ _ _, _ /\ _ => idtac | forall _ _ _ _ _ _ _ _ _, _ <-> _ => idtac | forall _ _ _ _ _ _ _ _ _ _, _ =>
-  match P with | forall _ _ _ _ _ _ _ _ _ _, _ /\ _ => idtac | forall _ _ _ _ _ _ _ _ _ _, _ <-> _ => idtac | forall _ _ _ _ _ _ _ _ _ _ _, _ =>
-  match P with | forall _ _ _ _ _ _ _ _ _ _ _, _ /\ _ => idtac | forall _ _ _ _ _ _ _ _ _ _ _, _ <-> _ => idtac | forall _ _ _ _ _ _ _ _ _ _ _ _, _ =>
-  match P with | forall _ _ _ _ _ _ _ _ _ _ _ _, _ /\ _ => idtac | forall _ _ _ _ _ _ _ _ _ _ _ _, _ <-> _ => idtac | forall _ _ _ _ _ _ _ _ _ _ _ _ _, _ =>
-  match P with | forall _ _ _ _ _ _ _ _ _ _ _ _ _, _ /\ _ => idtac | forall _ _ _ _ _ _ _ _ _ _ _ _ _, _ <-> _ => idtac | forall _ _ _ _ _ _ _ _ _ _ _ _ _ _, _ =>
-  match P with | forall _ _ _ _ _ _ _ _ _ _ _ _ _ _, _ /\ _ => idtac | forall _ _ _ _ _ _ _ _ _ _ _ _ _ _, _ <-> _ => idtac | forall _ _ _ _ _ _ _ _ _ _ _ _ _ _ _, _ =>
-  match P with | forall _ _ _ _ _ _ _ _ _ _ _ _ _ _ _, _ /\ _ => idtac | forall _ _ _ _ _ _ _ _ _ _ _ _ _ _ _, _ <-> _ => idtac | forall _ _ _ _ _ _ _ _ _ _ _ _ _ _ _ _, _ =>
-  match P with | forall _ _ _ _ _ _ _ _ _ _ _ _ _ _ _ _, _ /\ _ => idtac | forall _ _ _ _ _ _ _ _ _ _ _ _ _ _ _ _, _ <-> _ => idtac | forall _ _ _ _ _ _ _ _ _ _ _ _ _ _ _ _ _, _ =>
-  match P with | forall _ _ _ _ _ _ _ _ _ _ _ _ _ _ _ _ _, _ /\ _ => idtac | forall _ _ _ _ _ _ _ _ _ _ _ _ _ _ _ _ _, _ <-> _ => idtac | forall _ _ _ _ _ _ _ _ _ _ _ _ _ _ _ _ _ _, _ =>
-  match P with | forall _ _ _ _ _ _ _ _ _ _ _ _ _ _ _ _ _ _, _ /\ _ => idtac | forall _ _ _ _ _ _ _ _ _ _ _ _ _ _ _ _ _ _, _ <-> _ => idtac | forall _ _ _ _ _ _ _ _ _ _ _ _ _ _ _ _ _ _ _, _ =>
-  match P with | forall _ _ _ _ _ _ _ _ _ _ _ _ _ _ _ _ _ _ _, _ /\ _ => idtac | forall _ _ _ _ _ _ _ _ _ _ _ _ _ _ _ _ _ _ _, _ <-> _ => idtac | forall _ _ _ _ _ _ _ _ _ _ _ _ _ _ _ _ _ _ _ _, _ =>
+  match P with | forall _ _ _ _ _ _ _ _ _, _ /\ _ => idtac | forall _ _ _ _ _ _ _ _ _, _ <-> _ => idtac | forall _ _ _ _ _ _ _ _ _ _, _ => 
+  match P with | forall _ _ _ _ _ _ _ _ _ _, _ /\ _ => idtac | forall _ _ _ _ _ _ _ _ _ _, _ <-> _ => idtac | forall _ _ _ _ _ _ _ _ _ _ _, _ => 
+  match P with | forall _ _ _ _ _ _ _ _ _ _ _, _ /\ _ => idtac | forall _ _ _ _ _ _ _ _ _ _ _, _ <-> _ => idtac | forall _ _ _ _ _ _ _ _ _ _ _ _, _ => 
+  match P with | forall _ _ _ _ _ _ _ _ _ _ _ _, _ /\ _ => idtac | forall _ _ _ _ _ _ _ _ _ _ _ _, _ <-> _ => idtac | forall _ _ _ _ _ _ _ _ _ _ _ _ _, _ => 
+  match P with | forall _ _ _ _ _ _ _ _ _ _ _ _ _, _ /\ _ => idtac | forall _ _ _ _ _ _ _ _ _ _ _ _ _, _ <-> _ => idtac | forall _ _ _ _ _ _ _ _ _ _ _ _ _ _, _ => 
+  match P with | forall _ _ _ _ _ _ _ _ _ _ _ _ _ _, _ /\ _ => idtac | forall _ _ _ _ _ _ _ _ _ _ _ _ _ _, _ <-> _ => idtac | forall _ _ _ _ _ _ _ _ _ _ _ _ _ _ _, _ => 
+  match P with | forall _ _ _ _ _ _ _ _ _ _ _ _ _ _ _, _ /\ _ => idtac | forall _ _ _ _ _ _ _ _ _ _ _ _ _ _ _, _ <-> _ => idtac | forall _ _ _ _ _ _ _ _ _ _ _ _ _ _ _ _, _ => 
+  match P with | forall _ _ _ _ _ _ _ _ _ _ _ _ _ _ _ _, _ /\ _ => idtac | forall _ _ _ _ _ _ _ _ _ _ _ _ _ _ _ _, _ <-> _ => idtac | forall _ _ _ _ _ _ _ _ _ _ _ _ _ _ _ _ _, _ => 
+  match P with | forall _ _ _ _ _ _ _ _ _ _ _ _ _ _ _ _ _, _ /\ _ => idtac | forall _ _ _ _ _ _ _ _ _ _ _ _ _ _ _ _ _, _ <-> _ => idtac | forall _ _ _ _ _ _ _ _ _ _ _ _ _ _ _ _ _ _, _ => 
+  match P with | forall _ _ _ _ _ _ _ _ _ _ _ _ _ _ _ _ _ _, _ /\ _ => idtac | forall _ _ _ _ _ _ _ _ _ _ _ _ _ _ _ _ _ _, _ <-> _ => idtac | forall _ _ _ _ _ _ _ _ _ _ _ _ _ _ _ _ _ _ _, _ => 
+  match P with | forall _ _ _ _ _ _ _ _ _ _ _ _ _ _ _ _ _ _ _, _ /\ _ => idtac | forall _ _ _ _ _ _ _ _ _ _ _ _ _ _ _ _ _ _ _, _ <-> _ => idtac | forall _ _ _ _ _ _ _ _ _ _ _ _ _ _ _ _ _ _ _ _, _ => 
   match P with | forall _ _ _ _ _ _ _ _ _ _ _ _ _ _ _ _ _ _ _ _, _ /\ _ => idtac | forall _ _ _ _ _ _ _ _ _ _ _ _ _ _ _ _ _ _ _ _, _ <-> _ => idtac
   end end end end end end end end end end end end end end end end end end end end end.
 
@@ -367,8 +369,8 @@ Ltac check_hyp H := match H with _ => idtac end.
 (** Fail if hypothesis [H1] is not [H2]. *)
 Ltac check_equal H1 H2 := match H1 with H2 => idtac end.
 
-Ltac hdes :=
-  repeat match goal with | H : ?P |- _ => hdesF P; hdesHP H P end;
+Ltac hdes := 
+  repeat match goal with | H : ?P |- _ => hdesF P; hdesHP H P end; 
   unfold _HID_ in *.
 Ltac rdes H := red in H; des.
 Ltac rrdes H := move H at bottom; repeat red in H; des.
@@ -381,7 +383,7 @@ Tactic Notation "rrdes" ident(a) ident(b) :=
   (rrdes a; rrdes b).
 Tactic Notation "rrdes" ident(a) ident(b) ident(c) :=
   (rrdes a; rrdes b c).
-Tactic Notation "rrdes" ident(a) ident(b) ident(c) ident(d) :=
+Tactic Notation "rrdes" ident(a) ident(b) ident(c) ident(d) := 
   (rrdes a b; rrdes c d).
 
 (** Destruct the condition of an [if] expression occuring in the goal. *)
@@ -403,18 +405,18 @@ Ltac des_ifH H :=
 (* TODO tactics such as these should always do clean at the end to remove junk like [H : x = x] *)
 Ltac des_ifs :=
  clarify;
-  repeat
-    match goal with
-      | |- context[match ?x with _ => _ end] =>
+  repeat 
+    match goal with 
+      | |- context[match ?x with _ => _ end] => 
         match (type of x) with
           | { _ } + { _ } => destruct x; clarify
           | _ => let Heq := fresh "Heq" in destruct x as [] eqn: Heq; clarify
-        end
-      | H: context[ match ?x with _ => _ end ] |- _ =>
+        end 
+      | H: context[ match ?x with _ => _ end ] |- _ => 
         match (type of x) with
           | { _ } + { _ } => destruct x; clarify
           | _ => let Heq := fresh "Heq" in destruct x as [] eqn: Heq; clarify
-        end
+        end 
     end.
 
 Ltac desf := clarify; des; des_ifs.
@@ -428,7 +430,7 @@ Tactic Notation "dup" hyp(H) :=
 (* Tactic Notation "dup" hyp(H) tactic(tac) := *)
 (*   let H' := fresh H in assert (H' := H); tac H'. *)
 
-Ltac clarassoc := clarsimp; autorewrite with sflib sflibA in *; try done.
+Ltac clarassoc := clarsimp; autorewrite with sflib sflibA in *; try done. 
 
 Ltac sflib__hacksimp1 :=
    clarsimp;
@@ -498,6 +500,7 @@ Tactic Notation ":" tactic(c) :=
 
 (** Exploit an assumption (adapted from CompCert). *)
 
+(* commented because of connflict with compcert's exploit *)
 Ltac exploit x :=
     refine ((fun x y => y x) (x _ _ _ _ _ _ _ _ _ _ _ _ _ _ _ _ _ _ _ _ _ _ _ _ _ _ _ _ _ _ _ _ _ _) _)
  || refine ((fun x y => y x) (x _ _ _ _ _ _ _ _ _ _ _ _ _ _ _ _ _ _ _ _ _ _ _ _ _ _ _ _ _ _ _ _ _) _)
@@ -547,7 +550,7 @@ Ltac hexploit' x := let H := fresh in set (H := x); clear H; eapply mp; [eapply 
 
 (* set_prop N T A performs 'assert (A : P); [|set (N := T A)]' when T is a term of type (P -> _) *)
 
-Ltac set_prop N T A :=
+Ltac set_prop N T A := 
   let b := fresh in let ty := type of T in
   match ty with (forall (_:?P), _) => assert (A: P); [|set (N := T A)] end.
 
@@ -567,7 +570,7 @@ Tactic Notation "induction" "[" ident_list(y) "]" ident(x) "[" ident(z) "]"  :=
 
 Tactic Notation "induct" ident(x) := induction x; hacksimp.
 
-Tactic Notation "induct" ident(x) "[" ident(z) "]" :=
+Tactic Notation "induct" ident(x) "[" ident(z) "]" := 
   induction x; destruct z; hacksimp.
 
 Tactic Notation "induct" "[" ident_list(y) "]" ident(x)  :=
@@ -578,32 +581,32 @@ Tactic Notation "induct" "[" ident_list(y) "]" ident(x) "[" ident(z) "]"  :=
   first [ try (intros until x); revert y; induction x; destruct z; hacksimp
         | red; try (intros until x); revert y; induction x; destruct z; hacksimp ].
 
-Tactic Notation "edestructs" ident(a) :=
+Tactic Notation "edestructs" ident(a) := 
   (edestruct a).
-Tactic Notation "edestructs" ident(a) ident(b) :=
+Tactic Notation "edestructs" ident(a) ident(b) := 
   (edestruct a; edestruct b).
-Tactic Notation "edestructs" ident(a) ident(b) ident(c) :=
+Tactic Notation "edestructs" ident(a) ident(b) ident(c) := 
   (edestruct a; edestructs b c).
-Tactic Notation "edestructs" ident(a) ident(b) ident(c) ident(d) :=
+Tactic Notation "edestructs" ident(a) ident(b) ident(c) ident(d) := 
   (edestruct a; edestructs b c d).
-Tactic Notation "edestructs" ident(a) ident(b) ident(c) ident(d) ident(e) :=
+Tactic Notation "edestructs" ident(a) ident(b) ident(c) ident(d) ident(e) := 
   (edestruct a; edestructs b c d e).
 Tactic Notation "edestructs" ident(a) ident(b) ident(c) ident(d) ident(e) ident(f) :=
   (edestruct a; edestructs b c d e f).
-Tactic Notation "edestructs" ident(a) ident(b) ident(c) ident(d) ident(e) ident(f) ident(g) :=
+Tactic Notation "edestructs" ident(a) ident(b) ident(c) ident(d) ident(e) ident(f) ident(g) := 
   (edestruct a; edestructs b c d e f g).
 Tactic Notation "edestructs" ident(a) ident(b) ident(c) ident(d) ident(e) ident(f) ident(g) ident(h) :=
   (edestruct a; edestructs b c d e f g h).
-Tactic Notation "edestructs" ident(a) ident(b) ident(c) ident(d) ident(e) ident(f) ident(g) ident(h) ident(i) :=
+Tactic Notation "edestructs" ident(a) ident(b) ident(c) ident(d) ident(e) ident(f) ident(g) ident(h) ident(i) := 
   (edestruct a; edestructs b c d e f g h i).
-Tactic Notation "edestructs" ident(a) ident(b) ident(c) ident(d) ident(e) ident(f) ident(g) ident(h) ident(i) ident(j) :=
+Tactic Notation "edestructs" ident(a) ident(b) ident(c) ident(d) ident(e) ident(f) ident(g) ident(h) ident(i) ident(j) := 
   (edestruct a; edestructs b c d e f g h i j).
 
 Tactic Notation "destructs" ident(a) :=
   (destruct a).
-Tactic Notation "destructs" ident(a) ident(b) :=
+Tactic Notation "destructs" ident(a) ident(b) := 
   (destruct a; destruct b).
-Tactic Notation "destructs" ident(a) ident(b) ident(c) :=
+Tactic Notation "destructs" ident(a) ident(b) ident(c) := 
   (destruct a; destructs b c).
 Tactic Notation "destructs" ident(a) ident(b) ident(c) ident(d) :=
   (destruct a; destructs b c d).
@@ -613,19 +616,19 @@ Tactic Notation "destructs" ident(a) ident(b) ident(c) ident(d) ident(e) ident(f
   (destruct a; destructs b c d e f).
 Tactic Notation "destructs" ident(a) ident(b) ident(c) ident(d) ident(e) ident(f) ident(g) :=
   (destruct a; destructs b c d e f g).
-Tactic Notation "destructs" ident(a) ident(b) ident(c) ident(d) ident(e) ident(f) ident(g) ident(h) :=
+Tactic Notation "destructs" ident(a) ident(b) ident(c) ident(d) ident(e) ident(f) ident(g) ident(h) := 
   (destruct a; destructs b c d e f g h).
-Tactic Notation "destructs" ident(a) ident(b) ident(c) ident(d) ident(e) ident(f) ident(g) ident(h) ident(i) :=
+Tactic Notation "destructs" ident(a) ident(b) ident(c) ident(d) ident(e) ident(f) ident(g) ident(h) ident(i) := 
   (destruct a; destructs b c d e f g h i).
-Tactic Notation "destructs" ident(a) ident(b) ident(c) ident(d) ident(e) ident(f) ident(g) ident(h) ident(i) ident(j) :=
+Tactic Notation "destructs" ident(a) ident(b) ident(c) ident(d) ident(e) ident(f) ident(g) ident(h) ident(i) ident(j) := 
   (destruct a; destructs b c d e f g h i j).
 
 Tactic Notation "depdes" ident(_something_which_shold_not_occur_in_the_goal_) :=
-  (let _x_ := type of _something_which_shold_not_occur_in_the_goal_
+  (let _x_ := type of _something_which_shold_not_occur_in_the_goal_ 
    in dependent destruction _something_which_shold_not_occur_in_the_goal_).
-Tactic Notation "depdes" ident(a) ident(b) :=
+Tactic Notation "depdes" ident(a) ident(b) := 
   (depdes a; depdes b).
-Tactic Notation "depdes" ident(a) ident(b) ident(c) :=
+Tactic Notation "depdes" ident(a) ident(b) ident(c) := 
   (depdes a; depdes b c).
 Tactic Notation "depdes" ident(a) ident(b) ident(c) ident(d) :=
   (depdes a; depdes b c d).
@@ -635,11 +638,11 @@ Tactic Notation "depdes" ident(a) ident(b) ident(c) ident(d) ident(e) ident(f) :
   (depdes a; depdes b c d e f).
 Tactic Notation "depdes" ident(a) ident(b) ident(c) ident(d) ident(e) ident(f) ident(g) :=
   (depdes a; depdes b c d e f g).
-Tactic Notation "depdes" ident(a) ident(b) ident(c) ident(d) ident(e) ident(f) ident(g) ident(h) :=
+Tactic Notation "depdes" ident(a) ident(b) ident(c) ident(d) ident(e) ident(f) ident(g) ident(h) := 
   (depdes a; depdes b c d e f g h).
-Tactic Notation "depdes" ident(a) ident(b) ident(c) ident(d) ident(e) ident(f) ident(g) ident(h) ident(i) :=
+Tactic Notation "depdes" ident(a) ident(b) ident(c) ident(d) ident(e) ident(f) ident(g) ident(h) ident(i) := 
   (depdes a; depdes b c d e f g h i).
-Tactic Notation "depdes" ident(a) ident(b) ident(c) ident(d) ident(e) ident(f) ident(g) ident(h) ident(i) ident(j) :=
+Tactic Notation "depdes" ident(a) ident(b) ident(c) ident(d) ident(e) ident(f) ident(g) ident(h) ident(i) ident(j) := 
   (depdes a; depdes b c d e f g h i j).
 
 Tactic Notation "depgen" ident(x) := generalize dependent x.
@@ -667,7 +670,7 @@ Arguments __GUARD__ A a : simpl never.
 
 Tactic Notation "guard" constr(t) "in" hyp(H) := fold (__guard__ t) in H.
 Tactic Notation "guardH" hyp(H) := let t := type of H in guard t in H.
-Tactic Notation "guard" :=
+Tactic Notation "guard" :=  
   repeat match goal with [H: ?P |- _] =>
     try (match P with __guard__ _ => fail 2 end); guardH H
   end.
@@ -682,12 +685,12 @@ Ltac desH H := guard; unguardH H; des; unguard.
 
 Ltac splits :=
   intros; unfold NW;
-  repeat match goal with
+  repeat match goal with 
   | [ |- _ /\ _ ] => split
   end.
 Ltac esplits :=
   intros; unfold NW;
-  repeat match goal with
+  repeat match goal with 
   | [ |- @ex _ _ ] => eexists
   | [ |- _ /\ _ ] => split
   | [ |- @sig _ _ ] => eexists
@@ -696,10 +699,10 @@ Ltac esplits :=
   end.
 
 Tactic Notation "replace_all" constr(e) := repeat (
-  let X := fresh in assert (X: e) by (clarify; eauto; done);
+  let X := fresh in assert (X: e) by (clarify; eauto; done); 
   first [rewrite !X | setoid_rewrite X]; clear X).
 
-Lemma all_conj_dist: forall A (P Q: A -> Prop),
+Lemma all_conj_dist: forall A (P Q: A -> Prop), 
   (forall a, P a /\ Q a) -> (forall a, P a) /\ (forall a, Q a).
 Proof. intros; hdes; eauto. Qed.
 
@@ -741,7 +744,7 @@ Tactic Notation "rr" "in" hyp(H) := repeat red in H.
 
 Definition __mark__ A (a : A) : A := a.
 
-Tactic Notation "M" :=
+Tactic Notation "M" := 
   match goal with [|-?G] => fold (__mark__ G) end.
 
 Tactic Notation "Mdo" tactic(tac) :=
@@ -750,7 +753,7 @@ Tactic Notation "Mdo" tactic(tac) :=
 Tactic Notation "Mskip" tactic(tac) :=
   first [ match goal with [|- __mark__ _ ] => unfold __mark__ end | tac ].
 
-Tactic Notation "Mfirst" tactic(main) ";;" tactic(post) :=
+Tactic Notation "Mfirst" tactic(main) ";;" tactic(post) := 
    main; (Mdo (post; M)); (Mskip post).
 
 (* revert until *)
@@ -768,7 +771,7 @@ Ltac revert_until id :=
 Open Scope string_scope.
 Open Scope list_scope.
 
-Fixpoint beq_str (s1 s2: string) : bool :=
+Fixpoint beq_str (s1 s2: string) : bool := 
   match s1, s2 with
   | "", "" => true
   | String a s1', String b s2' => if Ascii.ascii_dec a b then beq_str s1' s2' else false
@@ -788,8 +791,8 @@ Definition _Evar_sflib_ (A:Type) (x:A) := x.
 
 Tactic Notation "hide_evar" int_or_var(n) := let QQ := fresh "QQ" in
   hget_evar n; intro;
-  lazymatch goal with [ H := ?X |- _] =>
-    set (QQ := X) in *; fold (_Evar_sflib_ X) in QQ; clear H
+  lazymatch goal with [ H := ?X |- _] => 
+    set (QQ := X) in *; fold (_Evar_sflib_ X) in QQ; clear H 
   end.
 
 Ltac hide_evars := repeat (hide_evar 1).
@@ -799,13 +802,13 @@ Ltac show_evars := repeat (match goal with [ H := @_Evar_sflib_ _ _ |- _ ] => un
 
 Ltac revert1 := match goal with [H: _|-_] => revert H end.
 
-Lemma eqimpl: forall P Q : Prop, P = Q -> P -> Q.
+Lemma eqimpl: forall P Q : Prop, P = Q -> P -> Q. 
 Proof. by i; subst; auto. Qed.
 
 Ltac ginduction H :=
   move H at top; revert_until H; induction H.
 
-Tactic Notation "greflgen" constr(t) "as" ident(g)  :=
+Tactic Notation "greflgen" constr(t) "as" ident(g)  := 
   let EQ := fresh "XEQ" in
   generalize (eq_refl t); generalize t at -2 as g
   ; intros ? EQ ?; revert EQ.
@@ -949,3 +952,391 @@ Tactic Notation "econsby" tactic(tac) :=
         |econstructor 19; (by tac)
         |econstructor 20; (by tac)
   ].
+
+
+(* Youngju's Tactics *)
+
+Lemma f_equal6 (A1 A2 A3 A4 A5 A6 B: Type) (f: A1 -> A2 -> A3 -> A4 -> A5 -> A6 -> B)
+      (x1 y1: A1) (EQ1: x1 = y1)
+      (x2 y2: A2) (EQ2: x2 = y2)
+      (x3 y3: A3) (EQ3: x3 = y3)
+      (x4 y4: A4) (EQ4: x4 = y4)
+      (x5 y5: A5) (EQ5: x5 = y5)
+      (x6 y6: A6) (EQ6: x6 = y6)
+  :
+    <<EQ: f x1 x2 x3 x4 x5 x6 = f y1 y2 y3 y4 y5 y6>>
+.
+Proof. subst. reflexivity. Qed.
+
+Lemma f_equal7 (A1 A2 A3 A4 A5 A6 A7 B: Type) (f: A1 -> A2 -> A3 -> A4 -> A5 -> A6 -> A7 -> B)
+      (x1 y1: A1) (EQ1: x1 = y1)
+      (x2 y2: A2) (EQ2: x2 = y2)
+      (x3 y3: A3) (EQ3: x3 = y3)
+      (x4 y4: A4) (EQ4: x4 = y4)
+      (x5 y5: A5) (EQ5: x5 = y5)
+      (x6 y6: A6) (EQ6: x6 = y6)
+      (x7 y7: A7) (EQ7: x7 = y7)
+  :
+    <<EQ: f x1 x2 x3 x4 x5 x6 x7 = f y1 y2 y3 y4 y5 y6 y7>>
+.
+Proof. subst. reflexivity. Qed.
+
+Lemma f_equal8 (A1 A2 A3 A4 A5 A6 A7 A8 B: Type) (f: A1 -> A2 -> A3 -> A4 -> A5 -> A6 -> A7 -> A8 -> B)
+      (x1 y1: A1) (EQ1: x1 = y1)
+      (x2 y2: A2) (EQ2: x2 = y2)
+      (x3 y3: A3) (EQ3: x3 = y3)
+      (x4 y4: A4) (EQ4: x4 = y4)
+      (x5 y5: A5) (EQ5: x5 = y5)
+      (x6 y6: A6) (EQ6: x6 = y6)
+      (x7 y7: A7) (EQ7: x7 = y7)
+      (x8 y8: A8) (EQ8: x8 = y8)
+  :
+    <<EQ: f x1 x2 x3 x4 x5 x6 x7 x8 = f y1 y2 y3 y4 y5 y6 y7 y8>>
+.
+Proof. subst. reflexivity. Qed.
+
+Ltac rpapply_raw H :=
+  first[erewrite f_equal8 | erewrite f_equal7 | erewrite f_equal6 | erewrite f_equal5 |
+        erewrite f_equal4 | erewrite f_equal3 | erewrite f_equal2 | erewrite f_equal];
+  [eapply H|..]; try reflexivity.
+
+Ltac is_applied_function TARGET :=
+  match TARGET with
+  | ?f ?x =>
+    idtac
+  | _ => fail
+  end
+.
+
+Ltac has_inside_strict A B :=
+  match A with
+  | context[B] => tryif (check_equal A B) then fail else idtac
+  | _ => fail
+  end
+.
+
+Ltac is_inside_others_body TARGET :=
+  tryif (repeat multimatch goal with
+                | [ |- context[?f ?x] ] =>
+                  (* idtac f; idtac x; *)
+                  tryif (has_inside_strict x TARGET)
+                  then fail 2
+                  else fail
+                end)
+  then fail
+  else idtac
+.
+
+Ltac on_leftest_function TAC :=
+  (* repeat *)
+  multimatch goal with
+  | [ |- context[?f ?x] ] =>
+    tryif (is_applied_function f)
+    then fail
+    else
+      tryif (is_inside_others_body f)
+      then fail
+      else TAC f
+  (* else TAC constr:(f) *)
+  (* TODO: What is the difference? *)
+  end
+.
+(* TODO: more cannonical way to get leftest function? *)
+(* I tried match reverse but it was not good *)
+(* TODO: I want to define "get_leftest_function" *)
+(* TODO: try tactic notation ? *)
+
+Ltac leftest_rpapply H :=
+  on_leftest_function ltac:(fun f =>
+     (idtac f; first
+                 (* TODO: why rewrite "with" doesn't work? *)
+                 [ erewrite (f_equal8 f)
+                 | erewrite (f_equal7 f)
+                 | erewrite (f_equal6 f)
+                 | erewrite (f_equal5 f)
+                 | erewrite (f_equal4 f)
+                 | erewrite (f_equal3 f)
+                 | erewrite (f_equal2 f)
+                 | erewrite (f_equal  f) | fail]); [ eapply H | .. ]; try reflexivity)
+.
+
+
+
+
+
+Ltac is_type x :=
+     match type of x with
+     | Type => idtac
+     | Set => idtac
+     | Prop => idtac (* TODO: needed? *)
+     | _ => fail
+     end.
+
+Ltac is_term_applied_function TARGET :=
+  match TARGET with
+  | ?f ?x =>
+    tryif (is_type x) then fail else idtac
+  | _ => fail
+  end
+.
+
+Ltac on_leftest_function_with_type TAC :=
+  (* repeat *)
+  multimatch goal with
+  | [ |- context[?f ?x] ] =>
+    tryif (is_term_applied_function f)
+    then fail
+    else
+      tryif (is_inside_others_body f)
+      then fail
+      else TAC f
+  end
+.
+
+Ltac rpapply H :=
+  on_leftest_function_with_type ltac:(fun f =>
+     (idtac f; first
+                 (* TODO: why rewrite "with" doesn't work? *)
+                 [ erewrite (f_equal8 f)
+                 | erewrite (f_equal7 f)
+                 | erewrite (f_equal6 f)
+                 | erewrite (f_equal5 f)
+                 | erewrite (f_equal4 f)
+                 | erewrite (f_equal3 f)
+                 | erewrite (f_equal2 f)
+                 | erewrite (f_equal  f) | fail]); [ eapply H | .. ]; try reflexivity)
+.
+
+
+
+(* it may run infinite loop *)
+Ltac all TAC :=
+  repeat multimatch goal with
+         | H: _ |- _ => TAC H
+         end;
+  try TAC
+.
+
+Ltac fold_in x H := fold x in H; fold x.
+
+Ltac fold_all x := all ltac:(fold_in x).
+
+Ltac clears x :=
+  repeat match goal with
+         | H: context[x] |- _ => clear H
+         | |- context[x] => fail 2 "It appears in the goal!"
+         end
+.
+
+
+
+Ltac hide_goal :=
+  match goal with
+  | [ |- ?G ] => let name := fresh "HIDDEN_GOAL" in
+                 set (name := G); replace G with name by reflexivity
+  (* ; move name at top <---- it breaks "unhide (hide X) = X". User may do it manually *)
+  end.
+Ltac unhide_goal :=
+  match goal with
+  | [ |- ?G ] => subst G
+  end.
+Ltac is_local_definition X :=
+  hide_goal;
+  tryif (unfold X)
+  then (unhide_goal)
+  else (unhide_goal; fail)
+.
+Ltac negate TAC := tryif TAC then fail else idtac.
+Ltac clear_unused :=
+  repeat multimatch goal with
+         | [H: ?T |- _] =>
+           negate ltac:(is_local_definition H);
+           match (type of T) with
+           | Prop => idtac
+           | _ => try clear H
+           end
+         end
+.
+Goal let x := 0 in forall n: nat, False.
+Proof.
+  intros.
+  clear_unused.
+Abort.
+
+(* TODO: Currently I use "is_local_definition" filter, but it may replaced with checking if it is Prop *)
+Ltac clear_tautology :=
+  repeat multimatch goal with
+         | [H: ?A = ?B, H2: ?B = ?A |- _] => clear H2
+         (* | [H: True |- _] => clear H *) (* clear_universal_truth takes care of this now *)
+         | [H: ?X, H2: ?X |- _] =>
+           negate ltac:(is_local_definition H2);
+           clear H2
+         (* | [H: ?A = ?A |- _] => clear H *) (* clear_universal_truth takes care of this now *)
+         end
+.
+
+Ltac clear_reducible_truth :=
+  let smart_tac := ss in
+  repeat multimatch goal with
+         | [H: ?P |- _ ] =>
+           match (type of P) with
+           | Prop =>
+             let temp := fresh "temp" in
+             tryif assert(temp: P) by (clear H; smart_tac)
+             (* check if it is reducible from other premises *)
+             then clear temp; clear H
+             else idtac
+           | _ => idtac
+           end
+         end
+.
+
+Ltac clear_universal_truth :=
+  let smart_tac := ss in
+  repeat multimatch goal with
+         | [H: ?P |- _ ] =>
+           match (type of P) with
+           | Prop =>
+             let temp := fresh "temp" in
+             tryif assert(temp: P) by (all clear; smart_tac)
+             (* check if it is reducible without any premise *)
+             then clear temp; clear H
+             else idtac
+           | _ => idtac
+           end
+         end
+.
+
+Ltac clear_tac := repeat (clear_unused; clear_tautology; clear_universal_truth).
+
+Ltac des_ifs_safe_aux TAC :=
+  TAC;
+  repeat
+    multimatch goal with
+    | |- context[match ?x with _ => _ end] =>
+      match (type of x) with
+      | { _ } + { _ } => destruct x; TAC; []
+      | _ => let Heq := fresh "Heq" in destruct x as [] eqn: Heq; TAC; []
+      end
+    | H: context[ match ?x with _ => _ end ] |- _ =>
+      match (type of x) with
+      | { _ } + { _ } => destruct x; TAC; []
+      | _ => let Heq := fresh "Heq" in destruct x as [] eqn: Heq; TAC; []
+      end
+    end.
+Tactic Notation "des_ifs_safe" := des_ifs_safe_aux clarify.
+Tactic Notation "des_ifs_safe" tactic(TAC) := des_ifs_safe_aux TAC.
+
+Ltac abstr_aux x var_name :=
+  let hyp_name := fresh "abstr_hyp_name" in
+  remember x as var_name eqn:hyp_name; clear hyp_name
+.
+
+Tactic Notation "abstr" constr(H) := let var_name := fresh "abstr_var_name" in abstr_aux H var_name.
+Tactic Notation "abstr" constr(H) ident(var_name) := abstr_aux H var_name.
+
+Hint Rewrite
+     andb_true_iff andb_false_iff
+     orb_true_iff orb_false_iff
+     negb_true_iff negb_false_iff
+
+     andb_true_r andb_true_l andb_false_r andb_false_l
+     orb_true_r orb_true_l orb_false_r orb_false_l
+     negb_andb negb_orb negb_involutive
+  : simpl_bool.
+
+Ltac simpl_bool := unfold Datatypes.is_true; unfold is_true;  autorewrite with simpl_bool in *.
+
+Ltac des_safe_aux TAC :=
+  TAC;
+  repeat (des1; TAC; [])
+.
+
+Tactic Notation "des_safe" := des_safe_aux clarify.
+Tactic Notation "des_safe" tactic(TAC) := des_safe_aux TAC.
+
+Definition admit (excuse: String.string) {T: Type} : T.  Admitted.
+Tactic Notation "admit" constr(excuse) := idtac excuse; exact (admit excuse).
+
+(* Copied from SoftwareFoundations - LibTactics.v *)
+(* ---------------------------------------------------------------------- *)
+(** ** Generalization *)
+
+(** [gen X1 .. XN] is a shorthand for calling [generalize dependent]
+    successively on variables [XN]...[X1]. Note that the variables
+    are generalized in reverse order, following the convention of
+    the [generalize] tactic: it means that [X1] will be the first
+    quantified variable in the resulting goal. *)
+
+Tactic Notation "gen" ident(X1) :=
+  generalize dependent X1.
+Tactic Notation "gen" ident(X1) ident(X2) :=
+  gen X2; gen X1.
+Tactic Notation "gen" ident(X1) ident(X2) ident(X3) :=
+  gen X3; gen X2; gen X1.
+Tactic Notation "gen" ident(X1) ident(X2) ident(X3) ident(X4)  :=
+  gen X4; gen X3; gen X2; gen X1.
+Tactic Notation "gen" ident(X1) ident(X2) ident(X3) ident(X4) ident(X5) :=
+  gen X5; gen X4; gen X3; gen X2; gen X1.
+Tactic Notation "gen" ident(X1) ident(X2) ident(X3) ident(X4) ident(X5)
+ ident(X6) :=
+  gen X6; gen X5; gen X4; gen X3; gen X2; gen X1.
+Tactic Notation "gen" ident(X1) ident(X2) ident(X3) ident(X4) ident(X5)
+ ident(X6) ident(X7) :=
+  gen X7; gen X6; gen X5; gen X4; gen X3; gen X2; gen X1.
+Tactic Notation "gen" ident(X1) ident(X2) ident(X3) ident(X4) ident(X5)
+ ident(X6) ident(X7) ident(X8) :=
+  gen X8; gen X7; gen X6; gen X5; gen X4; gen X3; gen X2; gen X1.
+Tactic Notation "gen" ident(X1) ident(X2) ident(X3) ident(X4) ident(X5)
+ ident(X6) ident(X7) ident(X8) ident(X9) :=
+  gen X9; gen X8; gen X7; gen X6; gen X5; gen X4; gen X3; gen X2; gen X1.
+Tactic Notation "gen" ident(X1) ident(X2) ident(X3) ident(X4) ident(X5)
+ ident(X6) ident(X7) ident(X8) ident(X9) ident(X10) :=
+  gen X10; gen X9; gen X8; gen X7; gen X6; gen X5; gen X4; gen X3; gen X2; gen X1.
+
+(* ---------------------------------------------------------------------- *)
+
+Ltac exists_prop PROP :=
+  tryif
+    (repeat multimatch goal with
+            | [H: PROP |- _ ] => (* idtac "Found!"; idtac H; *) fail 2
+            end)
+  then fail
+  else idtac
+.
+
+Ltac propagate_eq :=
+  repeat (multimatch goal with
+          | [H1: ?A = ?B, H2: ?B = ?C |- _ ] =>
+            tryif (check_equal A C)
+            then fail
+            else
+              tryif (exists_prop (A = C) + exists_prop (C = A))
+              then idtac
+              else
+                let name := fresh "EQ_CLOSURE_TAC" in
+                hexploit eq_trans; [exact H1|exact H2|]; intro name
+          | [H1: ?B = ?A, H2: ?B = ?C |- _ ] =>
+            tryif (check_equal A C)
+            then fail
+            else
+              tryif (exists_prop (A = C) + exists_prop (C = A))
+              then idtac
+              else
+                let name := fresh "EQ_CLOSURE_TAC" in
+                hexploit eq_trans; [exact (eq_sym H1)|exact H2|]; intro name
+          end)
+.
+
+(* get equality's transitive closure *)
+(* TODO: it checks equality too naive way; "(0, 1).fst != 0" here. *)
+Ltac eq_closure_tac :=
+  repeat (propagate_eq; clarify); clear_tac
+.
+
+Ltac rev_all TAC :=
+  repeat multimatch reverse goal with
+         | H: _ |- _ => TAC H
+         end;
+  try TAC
+.
